cedar-dafny/pe/soundness.dfy
@@ -1,23 +1,23 @@
 include "def.dfy"
-include "interpretation.dfy"
+include "environment.dfy"
 include "engine.dfy"
 include "../def/core.dfy"
 include "../def/engine.dfy"
 
 module pe.soundness {
   import opened definition
-  import opened interpretation
+  import opened environment
   import opened engine
   import ce = def.engine
   import def.core
 
-  lemma PEIsSound(e: definition.Expr, q: core.Request, s: core.EntityStore, Q: definition.Request, S: definition.EntityStore, I: Interpretation)
-    requires I.wellFormed()
-    requires var pr := I.replaceUnknownInRequest(Q); pr.Some? && pr.value == q
-    requires var ps := I.replaceUnknownInEntityStore(S); ps.Some? && ps.value == s
+  lemma PEIsSound(e: definition.Expr, q: core.Request, s: core.EntityStore, Q: definition.Request, S: definition.EntityStore, env: Environment)
+    requires env.wellFormed()
+    requires var pr := env.replaceUnknownInRequest(Q); pr.Some? && pr.value == q
+    requires var ps := env.replaceUnknownInEntityStore(S); ps.Some? && ps.value == s
     ensures var peRes := PartialEvaluator(Q, S).interpret(e);
             // If PE succeeds, then evaluating the residual and evaluating the original expression with the same unknown to value mappings should agree.
-            (peRes.Ok? ==> ce.Evaluator(q, s).interpret(I.replaceUnknownInExpr(e)) == I.interpret(peRes.value)) &&
+            (peRes.Ok? ==> ce.Evaluator(q, s).interpret(env.replaceUnknownInExpr(e)) == env.interpret(peRes.value)) &&
             // If PE fails, then evaluating the original expression with any uknown to value mappings should fail.
-            (peRes.Err? ==> ce.Evaluator(q, s).interpret(I.replaceUnknownInExpr(e)).Err?)
+            (peRes.Err? ==> ce.Evaluator(q, s).interpret(env.replaceUnknownInExpr(e)).Err?)
 }
